test/Server.fst
@@ -1,11 +1,11 @@
 module Server
 
-module B = FStar.Buffer
+module B = LowStar.Buffer
+module M = LowStar.Modifies
 module U32 = FStar.UInt32
 
-open C
-open FStar.Buffer
 open FStar.HyperStack.ST
+open LowStar.BufferOps
 
 module HS = FStar.HyperStack
 module ST = FStar.HyperStack.ST
@@ -16,11 +16,11 @@ type pointer t =
 type server_state =
   pointer U32.t
 
-let zero_terminated (h: HS.mem) (b: B.buffer char) =
+let zero_terminated (h: HS.mem) (b: B.buffer C.char) =
   let s = B.as_seq h b in
   B.length b > 0 /\
   B.length b <= FStar.UInt.max_int 32 /\
-  uint8_of_char (Seq.index s (B.length b - 1)) = 0uy
+  C.uint8_of_char (Seq.index s (B.length b - 1)) = 0uy
 
 #set-options "--z3rlimit 300"
 
@@ -28,14 +28,13 @@ let zero_terminated (h: HS.mem) (b: B.buffer char) =
   @summary: compares `b` and `s` for equality (without `s`'s trailing zero)
   @type: true
 *)
-val bufstrcmp (b: buffer char) (s: C.String.t): Stack bool
+val bufstrcmp (b: B.buffer C.char) (s: C.String.t): Stack bool
   (requires (fun h ->
     B.live h b /\
-    C.String.zero_free s /\
     zero_terminated h b))
   (ensures (fun h0 ret h1 ->
     B.live h1 b /\
-    modifies_0 h0 h1 /\
+    M.(modifies loc_none h0 h1) /\
     (ret = true ==> (
       let l = C.String.length s in
       B.length b >= l /\ (
@@ -48,18 +47,17 @@ let bufstrcmp b s =
   let h0 = ST.get () in
   push_frame ();
   let h1 = ST.get () in
-  let i: pointer U32.t = Buffer.create 0ul 1ul in
+  let i: pointer U32.t = B.alloca 0ul 1ul in
   let h2 = ST.get () in
-  assert (modifies_0 h1 h2);
   let inv h stopped =
     B.live h i /\ B.live h b /\
-    B.modifies_1 i h2 h /\ (
+    M.(modifies (loc_buffer i) h2 h) /\ (
     let i: U32.t = B.get h i 0 in
     U32.v i < B.length b /\ U32.v i < C.String.length s /\
     (forall (j: U32.t). {:pattern (B.get h b (U32.v j)) } U32.lt j i ==>
       B.get h b (U32.v j) = C.String.get s j) /\
     (if stopped then
-      C.String.get s i = char_of_uint8 0uy \/ C.String.get s i <> B.get h b (U32.v i)
+      C.String.get s i = C.char_of_uint8 0uy \/ C.String.get s i <> B.get h b (U32.v i)
     else
       True))
   in
@@ -69,10 +67,15 @@ let bufstrcmp b s =
   =
     let cb = b.(i.(0ul)) in
     let cs = C.String.get s i.(0ul) in
-    if cb <> cs || cs = char_of_uint8 0uy then
+    if cb <> cs || cs = C.char_of_uint8 0uy then
       true
     else begin
       let h = ST.get () in
+      assert (
+        let i: U32.t = B.get h i 0 in
+        U32.v i < C.String.length s - 1
+      );
+      assert (C.String.well_formed (C.String.v s));
       assert (
         let i: U32.t = B.get h i 0 in
         forall (j: U32.t). {:pattern (B.get h b (U32.v j)) } U32.lt j i ==>
@@ -95,9 +98,9 @@ let bufstrcmp b s =
     end
   in
   C.Loops.do_while inv body;
-  let r = C.String.get s (i.(0ul)) = char_of_uint8 0uy in
+  let r = C.String.get s (i.(0ul)) = C.char_of_uint8 0uy in
   let h3 = ST.get () in
-  assert (forall (b: buffer char) (i: nat{ i < B.length b }).
+  assert (forall (b: B.buffer C.char) (i: nat{ i < B.length b }).
     {:pattern (Seq.index (B.as_seq h3 b) i)}
     Seq.index (B.as_seq h3 b) i == B.get h3 b i);
   assert (forall (s: C.String.t) (i: nat { i < C.String.length s }).
@@ -121,8 +124,6 @@ let bufstrcmp b s =
   );
   pop_frame ();
   let h4 = ST.get () in
-  lemma_modifies_0_1' i h1 h2 h3;
-  modifies_popped_0 h0 h1 h3 h4;
   r
 
 
@@ -131,15 +132,14 @@ let bufstrcmp b s =
   @returns: the number of bytes written out in `b`
   @type: true
 *)
-assume val bufstrcpy (b: buffer char) (s: C.String.t): Stack U32.t
+assume val bufstrcpy (b: B.buffer C.char) (s: C.String.t): Stack U32.t
   (requires (fun h ->
     B.live h b /\
-    C.String.zero_free s /\
     B.length b >= C.String.length s - 1))
   (ensures (fun h0 ret h1 ->
     B.live h1 b /\
     B.length b >= C.String.length s /\
-    modifies_1 b h0 h1 /\
+    M.(modifies (loc_buffer b) h0 h1) /\
     U32.v ret = C.String.length s - 1 /\
     Seq.equal (Seq.slice (B.as_seq h1 b) 0 (U32.v ret)) (Seq.slice (C.String.v s) 0 (U32.v ret))))
 
@@ -149,11 +149,11 @@ assume val bufstrcpy (b: buffer char) (s: C.String.t): Stack U32.t
   @returns: the number of bytes written out in `dst`
   @type: true
 *)
-assume val print_u32 (dst: buffer char) (i: U32.t): Stack U32.t
+assume val print_u32 (dst: B.buffer C.char) (i: U32.t): Stack U32.t
   (requires (fun h ->
     B.live h dst /\ B.length dst >= 10))
   (ensures (fun h0 ret h1 ->
-    modifies_1 dst h0 h1 /\
+    M.(modifies (loc_buffer dst) h0 h1) /\
     U32.v ret <= 10 /\
     B.live h1 dst))
 
@@ -163,7 +163,7 @@ assume val print_u32 (dst: buffer char) (i: U32.t): Stack U32.t
   @returns: the number of bytes written out in `b1`
   @type: true
 *)
-assume val bufcpy (b1 b2: buffer char): Stack U32.t
+assume val bufcpy (b1 b2: B.buffer C.char): Stack U32.t
   (requires (fun h ->
     B.live h b1 /\ B.live h b2 /\
     zero_terminated h b2 /\
@@ -172,7 +172,7 @@ assume val bufcpy (b1 b2: buffer char): Stack U32.t
     B.live h1 b1 /\ B.live h1 b2 /\
     zero_terminated h1 b2 /\
     B.length b2 >= B.length b1 - 1 /\
-    modifies_1 b1 h0 h1 /\ (
+    M.(modifies (loc_buffer b1) h0 h1) /\ (
     U32.v ret < B.length b1 /\
     Seq.equal (Seq.slice (B.as_seq h1 b1) 0 (U32.v ret)) (Seq.slice (B.as_seq h1 b2) 0 (U32.v ret)))))
 
@@ -181,17 +181,11 @@ assume val bufcpy (b1 b2: buffer char): Stack U32.t
 unfold noextract
 let response_length = 65535
 
-let offset_zero_terminated h (b: buffer char) (i: U32.t):
-  Lemma
-    (requires (U32.v i < B.length b /\ zero_terminated h b))
-    (ensures (U32.v i < B.length b /\ zero_terminated h (B.offset b i)))
-    [ SMTPat (zero_terminated h b); SMTPat (B.offset b i) ] =
-  ()
 
 inline_for_extraction noextract
 let (!$) = C.String.of_literal
 
-val respond: (response: buffer char) -> (payload: buffer char) -> (payloadlen: U32.t) ->
+val respond: (response: B.buffer C.char) -> (payload: B.buffer C.char) -> (payloadlen: U32.t) ->
   Stack U32.t
     (requires (fun h0 ->
       B.length payload >= U32.v payloadlen /\
@@ -204,7 +198,7 @@ val respond: (response: buffer char) -> (payload: buffer char) -> (payloadlen: U
       B.live h1 response /\
       B.live h1 payload /\
       B.disjoint response payload /\
-      B.modifies_1 response h0 h1 /\
+      M.(modifies (M.loc_buffer response) h0 h1) /\
       U32.v n <= 128 + U32.v payloadlen
     ))
 
@@ -215,36 +209,36 @@ let respond response payload payloadlen =
   let response = B.offset response n2 in
   let n3 = bufstrcpy response !$"\r\nContent-Type: text/html; charset=utf-8\r\n\r\n" in
   let response = B.offset response n3 in
-  let t = Buffer.blit payload 0ul response 0ul payloadlen in
+  let t = blit payload 0ul response 0ul payloadlen in
   U32.(n1 +^ n2 +^ n3 +^ payloadlen)
 
 #set-options "--max_ifuel 0"
 
-let respond_index (response: buffer char): Stack U32.t
+let respond_index (response: B.buffer C.char): Stack U32.t
   (requires (fun h0 ->
     B.live h0 response /\
     B.length response >= 256))
   (ensures (fun h0 n h1 ->
     B.live h1 response /\
-    B.modifies_1 response h0 h1 /\
+    M.(modifies (loc_buffer response) h0 h1) /\
     U32.v n <= 256)) =
   push_frame ();
-  let payload = Buffer.create (char_of_uint8 0uy) 256ul in
+  let payload = B.alloca (C.char_of_uint8 0uy) 256ul in
   let payloadlen = bufstrcpy payload !$"<html><body>Hello world</body></html>" in
   let n = respond response payload payloadlen in
   pop_frame ();
   n
 
-let respond_stats (response: buffer char) (state: U32.t): Stack U32.t
+let respond_stats (response: B.buffer C.char) (state: U32.t): Stack U32.t
   (requires (fun h0 ->
     B.live h0 response /\
     B.length response >= 256))
   (ensures (fun h0 n h1 ->
     B.live h1 response /\
-    B.modifies_1 response h0 h1 /\
+    M.(modifies (loc_buffer response) h0 h1) /\
     U32.v n <= 256)) =
   push_frame ();
-  let payload = Buffer.create (char_of_uint8 0uy) 256ul in
+  let payload = B.alloca (C.char_of_uint8 0uy) 256ul in
   let n1 = bufstrcpy payload !$"<html>State = " in
   let next = B.offset payload n1 in
   let n2 = print_u32 next state in
@@ -254,16 +248,16 @@ let respond_stats (response: buffer char) (state: U32.t): Stack U32.t
   pop_frame ();
   n
 
-let respond_404 (response: buffer char): Stack U32.t
+let respond_404 (response: B.buffer C.char): Stack U32.t
   (requires (fun h0 ->
     B.live h0 response /\
     B.length response >= 512))
   (ensures (fun h0 n h1 ->
     B.live h1 response /\
-    B.modifies_1 response h0 h1 /\
+    M.(modifies (loc_buffer response) h0 h1) /\
     U32.v n <= 512)) =
   push_frame ();
-  let payload = Buffer.create (char_of_uint8 0uy) 256ul in
+  let payload = B.alloca (C.char_of_uint8 0uy) 256ul in
   let payloadlen = bufstrcpy payload !$"<html>Page not found</html>" in
   let n1 = bufstrcpy response !$"HTTP/1.1 404 Not Found\r\nConnection: closed\r\nContent-Length:" in
   let response = B.offset response n1 in
@@ -271,7 +265,7 @@ let respond_404 (response: buffer char): Stack U32.t
   let response = B.offset response n2 in
   let n3 = bufstrcpy response !$"\r\nContent-Type: text/html; charset=utf-8\r\n\r\n" in
   let response = B.offset response n3 in
-  let t = Buffer.blit payload 0ul response 0ul payloadlen in
+  let t = blit payload 0ul response 0ul payloadlen in
   let n = U32.(n1+^n2+^n3+^payloadlen) in
   pop_frame ();
   n
@@ -283,7 +277,7 @@ let respond_404 (response: buffer char): Stack U32.t
   This is just to demonstrate some low-level style programming along with
   manipulation of strings.
 *)
-val server (state: server_state) (request response: buffer char):
+val server (state: server_state) (request response: B.buffer C.char):
   Stack U32.t
     (requires (fun h ->
       B.live h state /\ B.live h request /\ B.live h response /\
@@ -309,7 +303,7 @@ let server state request response =
 
     else
       // Bug of mine here: I was advancing by 5 instead of 4...!
-      let request = Buffer.offset request 4ul in
+      let request = B.offset request 4ul in
 
       if bufstrcmp request !$"/ " then
         respond_index response
